Partially verifying taint poly

src/arch/x64/X64.Vale.Decls_i.fsti
@@ -296,10 +296,12 @@ unfold let modifies_buffer_2 (b1 b2:M.buffer64) (h1 h2:M.mem) =modifies_mem (M.l
 unfold let modifies_buffer128 (b:M.buffer128) (h1 h2:M.mem) = modifies_mem (loc_buffer b) h1 h2
 unfold let modifies_buffer128_2 (b1 b2:M.buffer128) (h1 h2:M.mem) = modifies_mem (M.loc_union (loc_buffer b1) (loc_buffer b2)) h1 h2
 
-let validSrcAddrs64 (m:M.mem) (addr:int) (b:M.buffer64) (len:int) =
+let validSrcAddrs64 (m:M.mem) (addr:int) (b:M.buffer64) (len:int) (memTaint:map int taint) (t:taint) =
     buffer_readable m b /\
     len <= buffer_length b /\
-    M.buffer_addr b m == addr
+    M.buffer_addr b m == addr /\ 
+    (forall a. 0 <= a && a <= len ==>
+      memTaint.[addr + 8 `op_Multiply` a] == t)
 
 unfold 
 let validDstAddrs64 = validSrcAddrs64
